src/ConcurrentFS.v
@@ -16,7 +16,9 @@ Require Import HomeDirProtocol.
 Require Import RelationClasses.
 
 Record FsParams :=
-  { fsmem: ident; (* : memsstate *)
+  { cache: ident; (* : Cache *)
+    vdisk: ident; (* : Disk *)
+    fsmem: ident; (* : memsstate *)
     fstree: ident; (* : dirtree *)
     fshomedirs: ident; (* thread_homes *)
     }.
@@ -24,7 +26,6 @@ Record FsParams :=
 Section ConcurrentFS.
 
   Variable fsxp: fs_xparams.
-  Variable CP:CacheParams.
   Variable P:FsParams.
 
   Definition fs_rep vd hm mscs tree :=
@@ -37,9 +38,12 @@ Section ConcurrentFS.
   Definition fs_invariant d hm tree (homedirs: thread_homes) : heappred :=
     (fstree P |-> abs tree *
      fshomedirs P |-> abs homedirs *
-     exists mscs vd, CacheRep CP d empty_writebuffer vd vd *
-                fsmem P |-> val mscs *
-                [[ fs_rep vd hm mscs tree ]])%pred.
+     exists c vd mscs,
+       cache P |-> val c *
+       vdisk P |-> absMem vd *
+       [[ CacheRep d c vd ]] *
+       fsmem P |-> val mscs *
+       [[ fs_rep vd hm mscs tree ]])%pred.
 
   Definition fs_guarantee tid (sigma sigma':Sigma) :=
     exists tree tree' homedirs,
@@ -203,32 +207,25 @@ Section ConcurrentFS.
 
   Definition OptimisticProg T :=
     memstate ->
-    LockState -> WriteBuffer ->
-    cprog (Result (memstate * T) * WriteBuffer).
+    LockState -> Cache ->
+    cprog (Result (memstate * T) * Cache).
 
   (* Execute p assuming it is read-only. This program could distinguish between
   failures that require filling the cache [Failure (CacheMiss a)] and failures
   that require upgrading to a write lock [Failure WriteRequired], but currently
-  does not do so. *)
+  does not do so. This would be useful to help the interpreter schedule reads
+  (by waiting on address a before re-scheduling, for example). *)
   Definition readonly_syscall T (p: OptimisticProg T) : cprog (SyscallResult T) :=
-    _ <- GetReadLock;
-      mscs <- Get memstate (fsmem P);
+    do '(c, mscs) <- Read2 Cache (cache P) memstate (fsmem P);
       (* for read-only syscalls, the returned write buffer is always the same
        as the input *)
-      do '(r, _) <- p mscs ReadLock empty_writebuffer;
+      do '(r, _) <- p mscs Free c;
       match r with
       | Success (ms', r) =>
-        l <- UpgradeReadLock;
-          _ <- if lock_dec l WriteLock then
-                _ <- Assgn (fsmem P) ms';
-                  _ <- Unlock;
-                  Ret tt
-              else
-                _ <- ReleaseReadLock;
-                Ret tt;
-          Ret (Done r)
+        (* TODO: if FSCQ code tells us to, restart with write lock to commit
+        memstate *)
+        Ret (Done r)
       | Failure e =>
-        _ <- ReleaseReadLock;
         match e with
         | Unsupported => Ret SyscallFailed
         | _ => Ret TryAgain
@@ -246,19 +243,23 @@ Section ConcurrentFS.
     cprog (SyscallResult T) :=
     retry guard
           (_ <- GetWriteLock;
-             m <- Get _ (fsmem P);
-             do '(r, wb) <- p m WriteLock empty_writebuffer;
+             do '(c, mscs) <- Read2 Cache (cache P) memstate (fsmem P);
+             do '(r, c) <- p mscs WriteLock c;
              match r with
              | Success (ms', r) =>
-               _ <- CacheCommit CP wb;
-                 _ <- Assgn (fsmem P) ms';
-                 _ <- GhostUpdate (fstree P) (fun _ => update);
+               _ <- Assgn2_mem_abs (Make_assgn2
+                                     (cache P) c
+                                     (fsmem P) ms'
+
+                                     (* TODO: how do we incorporate the new
+                                 cache into the virtual disk? *)
+                                     (vdisk P) (fun _ (vd:Disk) => vd)
+                                     (fstree P) (fun _ => update));
                  _ <- Unlock;
                  Ret (Done r)
              | Failure e =>
                match e with
                | CacheMiss a =>
-                 _ <- CacheAbort;
                    _ <- Unlock;
                    (* TODO: [Yield a] here when the noop Yield is added *)
                    Ret TryAgain
@@ -280,49 +281,43 @@ Section ConcurrentFS.
   Record FsSpecParams T :=
     { fs_pre : dirtree -> Prop;
       fs_post : T -> Prop;
-      fs_mscs_R : memstate -> memstate -> Prop;
       fs_dirup : dirtree -> dirtree; }.
 
   Definition FsSpec A T := A -> FsSpecParams T.
 
   Definition fs_spec A T (fsspec: FsSpec A T) :
-    memstate -> LockState ->
-    Spec _ (Result (memstate * T) * WriteBuffer) :=
-    fun mscs l '(F, vd0, vd, tree, a) '(sigma_i, sigma) =>
+    memstate -> LockState -> Cache ->
+    Spec _ (Result (memstate * T) * Cache) :=
+    fun mscs l c '(F, d, vd, tree, a) sigma =>
       {| precondition :=
-           (F * CacheRep CP (Sigma.disk sigma) empty_writebuffer vd0 vd)%pred (Sigma.mem sigma) /\
+           F (Sigma.mem sigma) /\
+           CacheRep d c vd /\
            fs_rep vd (Sigma.hm sigma) mscs tree /\
            fs_pre (fsspec a) tree /\
-           Sigma.l sigma = l /\
-           ReadPermission l;
+           Sigma.l sigma = l;
          postcondition :=
-           fun '(sigma_i', sigma') '(r, wb') =>
+           fun sigma' '(r, c') =>
              exists vd',
-             (F * CacheRep CP (Sigma.disk sigma) empty_writebuffer vd0 vd')%pred (Sigma.mem sigma') /\
-             Sigma.l sigma' = l /\
-             (l = ReadLock -> vd' = vd) /\
-             match r with
-             | Success (mscs', r) =>
-               fs_post (fsspec a) r /\
-               fs_mscs_R (fsspec a) mscs mscs' /\
-               fs_rep vd' (Sigma.hm sigma') mscs' (fs_dirup (fsspec a) tree)
-             | Failure e =>
-               (l = WriteLock -> e <> WriteRequired) /\
-               fs_rep vd (Sigma.hm sigma') mscs tree
-             end /\
-             hashmap_le (Sigma.hm sigma) (Sigma.hm sigma') /\
-             sigma_i' = sigma_i; |}.
+               F (Sigma.mem sigma') /\
+               let d' := if CanWrite l then Sigma.disk sigma' else d in
+               CacheRep d' c' vd' /\
+               Sigma.l sigma' = Sigma.l sigma /\
+               (l = Free -> vd' = vd) /\
+               (l = Free -> c' = c) /\
+               match r with
+               | Success (mscs', r) =>
+                 fs_post (fsspec a) r /\
+                 fs_rep vd' (Sigma.hm sigma') mscs' (fs_dirup (fsspec a) tree)
+               | Failure e =>
+                 (l = WriteLock -> e <> WriteRequired) /\
+                 fs_rep vd (Sigma.hm sigma') mscs tree
+               end /\
+               hashmap_le (Sigma.hm sigma) (Sigma.hm sigma') ; |}.
 
   Definition precondition_stable A T (fsspec: FsSpec A T) homes tid :=
     forall a tree tree', fs_pre (fsspec a) tree ->
                     homedir_rely tid homes tree tree' ->
                     fs_pre (fsspec a) tree'.
-
-  Definition mscs_nocommit A T (fsspec: FsSpec A T) :=
-    forall a mscs mscs',
-      fs_mscs_R (fsspec a) mscs mscs' ->
-      (forall d tree hm, fs_rep d tree mscs' hm ->
-                    fs_rep d tree mscs hm).
 
   Lemma precondition_stable_rely_fwd : forall A T (spec: FsSpec A T) tid a
                                      sigma tree homedirs sigma',
@@ -346,15 +341,14 @@ Section ConcurrentFS.
 
   Definition readonly_spec A T (fsspec: FsSpec A T) tid :
     Spec _ (SyscallResult T) :=
-    fun '(tree, homedirs, a) '(sigma_i, sigma) =>
+    fun '(tree, homedirs, a) sigma =>
       {| precondition :=
            (fs_invariant (Sigma.disk sigma) (Sigma.hm sigma) tree homedirs) (Sigma.mem sigma) /\
            Sigma.l sigma = Free /\
            fs_pre (fsspec a) tree /\
-           precondition_stable fsspec homedirs tid /\
-           mscs_nocommit fsspec;
+           precondition_stable fsspec homedirs tid;
          postcondition :=
-           fun '(sigma_i', sigma') r =>
+           fun sigma' r =>
              (fs_invariant (Sigma.disk sigma') (Sigma.hm sigma') tree homedirs) (Sigma.mem sigma') /\
              Rely fs_guarantee tid sigma sigma' /\
              Sigma.l sigma' = Free /\
@@ -362,8 +356,7 @@ Section ConcurrentFS.
              | Done v => fs_post (fsspec a) v
              | TryAgain => True
              | SyscallFailed => True
-             end /\
-             fs_guarantee tid sigma_i' sigma'|}.
+             end |}.
 
   Lemma fs_rep_hashmap_incr : forall vd tree mscs hm hm',
       fs_rep vd hm mscs tree ->
@@ -378,95 +371,17 @@ Section ConcurrentFS.
 
   Hint Resolve fs_rep_hashmap_incr.
 
-  Theorem readonly_syscall_ok : forall T (p: OptimisticProg T) A (fsspec: FsSpec A T) tid,
+  Theorem readonly_syscall_ok : forall T (p: OptimisticProg T) A (fsspec: FsSpec A T) c tid,
       (forall mscs, cprog_spec fs_guarantee tid
-                          (fs_spec fsspec mscs ReadLock)
-                          (p mscs ReadLock empty_writebuffer)) ->
+                          (fs_spec fsspec mscs Free c)
+                          (p mscs Free c)) ->
       cprog_spec fs_guarantee tid
                  (readonly_spec fsspec tid) (readonly_syscall p).
   Proof.
-    intros.
-    unfold readonly_syscall.
-
-    step.
-    destruct st as [sigma_i sigma]; simpl in *.
-    destruct a as ((tree & homedirs) & a); simpl in *.
-    intuition eauto.
-
-    step.
-    deex.
-    destruct sigma'; simpl; auto.
-
-    match goal with
-    | [ H: Rely fs_guarantee _ _ _ |- _ ] =>
-      pose proof H;
-        eapply precondition_stable_rely_fwd in H; eauto;
-          deex
-    end.
-    unfold fs_invariant in H9.
-    (* need to deex mscs inside fs_invariant - should write an unfold rule that moves the existential to the top *)
-    descend; simpl in *; intuition eauto.
-    unfold fs_invariant in *.
-    SepAuto.pred_apply; SepAuto.cancel.
-    Show Existentials.
-    instantiate (1 := mscs).
-
-    step_using ltac:(apply H).
-    eexists; simpl; intuition eauto.
-
-    unfold fs_invariant in *; intuition eauto.
-    destruct sigma'; simpl in *; eauto.
-    destruct sigma'; simpl in *; eauto.
-    unfold fs_invariant in *; intuition eauto.
-    destruct sigma'; simpl in *; eauto.
-    unfold get_fstree in *; destruct sigma'; simpl in *; eauto.
-
-    step.
-    intuition eauto.
-    match goal with
-    | [ u:unit |- _ ] => destruct u
-    end.
-
-    assert (fs_invariant (Sigma.set_l sigma0 Free)).
-    unfold fs_invariant, locally_modified, seq_disk, get_fstree, get_fsmem in *;
-      destruct sigma', sigma0; simpl in *; intuition eauto.
-    repeat match goal with
-           | [ H: _ = _ |- _ ] =>
-             progress rewrite H in *
-           end.
-    eauto.
-
-    assert (fs_guarantee tid sigma' (Sigma.set_l sigma0 Free)).
-    unfold fs_guarantee, get_homedirs, get_fstree, locally_modified in *;
-      destruct sigma', sigma0; simpl in *; intuition eauto.
-    match goal with
-    | [ |- homedir_guarantee _ _ ?tree ?tree' ] =>
-      replace tree' with tree by congruence;
-        reflexivity
-    end.
-    congruence.
-
-    assert (fs_guarantee tid (Sigma.set_l sigma' ReadLock) (Sigma.set_l sigma0 Free)).
-    destruct sigma'; simpl in *; eauto.
-
-    assert (Rely fs_guarantee tid sigma (Sigma.set_l sigma0 Free)).
-    eapply Rely_trans; eauto.
-    constructor.
-    exists (S tid); intuition.
-
-    destruct a0 as [(mscs & r) | ].
-    step.
-    intuition eauto.
-    destruct sigma0; simpl; auto.
-
-    destruct e; step; intuition eauto.
-    destruct sigma0; simpl; auto.
-    destruct sigma0; simpl; auto.
-    destruct sigma0; simpl; auto.
-  Qed.
+  Abort.
 
   Definition file_get_attr inum :=
-    retry_syscall (fun mscs => file_get_attr _ fsxp inum mscs)
+    retry_syscall (fun mscs => OptFS.file_get_attr fsxp inum mscs)
                   (fun tree => tree).
 
   Lemma exists_tuple : forall A B P,
@@ -488,151 +403,17 @@ Section ConcurrentFS.
            | _ => progress subst
            end.
 
-  Hint Extern 0 {{ CacheCommit _; _ }} => apply CacheCommit_ok : prog.
-  Hint Extern 0 {{ CacheAbort; _ }} => apply CacheAbort_ok : prog.
-
-  Lemma locally_modified_fstree : forall sigma sigma',
-      locally_modified sigma sigma' ->
-      get_fstree sigma' = get_fstree sigma.
-  Proof.
-    unfold get_fstree, locally_modified; intros.
-    destruct sigma, sigma'; simpl in *; intuition congruence.
-  Qed.
-
-  Lemma locally_modified_fsmem : forall sigma sigma',
-      locally_modified sigma sigma' ->
-      get_fsmem (Sigma.mem sigma') = get_fsmem (Sigma.mem sigma).
-  Proof.
-    unfold get_fsmem, locally_modified; intros.
-    destruct sigma, sigma'; simpl in *; intuition congruence.
-  Qed.
-
-  Lemma locally_modified_homedirs : forall sigma sigma',
-      locally_modified sigma sigma' ->
-      get_homedirs sigma' = get_homedirs sigma.
-  Proof.
-    unfold get_homedirs, locally_modified; intros.
-    destruct sigma, sigma'; simpl in *; intuition congruence.
-  Qed.
-
-  Ltac learning :=
-    repeat match goal with
-           | [ H: locally_modified _ _ |- _ ] =>
-             learn that (locally_modified_fstree H)
-           | [ H: locally_modified _ _ |- _ ] =>
-             learn that (locally_modified_fsmem H)
-           | [ H: locally_modified _ _ |- _ ] =>
-             learn that (locally_modified_homedirs H)
-           | [ H: locally_modified _ _ |- _ ] =>
-             learn that (locally_modified_lock_preserved H)
-           | [ H: CacheRep empty_writebuffer _ |- _ ] =>
-             learn that (CacheRep_empty H)
-           end.
-
-  Lemma upd_fstree_id : forall up sigma,
-      (forall tree, up tree = tree) ->
-      upd_fstree up sigma = sigma.
-  Proof.
-    unfold upd_fstree.
-    destruct sigma, cache_other_s; simpl; intros.
-    rewrite H; auto.
-  Qed.
-
-  Lemma get_set_fsmem : forall m mscs,
-      get_fsmem (set_fsmem m mscs) = mscs.
-  Proof.
-    reflexivity.
-  Qed.
-
-  Lemma seq_disk_set_fsmem : forall d m mscs s hm l,
-      seq_disk (state d (set_fsmem m mscs) s hm l) = seq_disk (state d m s hm l).
-  Proof.
-    reflexivity.
-  Qed.
-
-  Lemma get_fstree_set_fsmem : forall d m mscs s hm l,
-      get_fstree (state d (set_fsmem m mscs) s hm l) = get_fstree (state d m s hm l).
-  Proof.
-    reflexivity.
-  Qed.
-
-  Hint Rewrite upd_fstree_id using solve [ auto ] : get_set.
-  Hint Rewrite get_set_fsmem seq_disk_set_fsmem get_fstree_set_fsmem : get_set.
-
-  Ltac simplify :=
-    repeat match goal with
-           | [ H: get_fstree _ = get_fstree _ |- _ ] =>
-             rewrite H in *
-           | _ => progress autorewrite with get_set
-           | _ => progress simpl
-           end.
-
-  Theorem opt_file_get_attr_ok : forall inum mscs l tid,
+  Theorem opt_file_get_attr_ok : forall inum mscs l tid c,
       cprog_spec fs_guarantee tid
                  (fs_spec (fun '(pathname, f) =>
                              {| fs_pre :=
                                   fun tree => find_subtree pathname tree = Some (TreeFile inum f);
                                 fs_post :=
                                   fun '(r, _) => r = BFILE.BFAttr f;
-                                fs_mscs_R :=
-                                  fun mscs mscs' => MSAlloc mscs' = MSAlloc mscs;
-                                fs_dirup := fun tree => tree |}) mscs l)
-                 (OptFS.file_get_attr _ fsxp inum mscs l empty_writebuffer).
+                                fs_dirup := fun tree => tree |}) mscs l c)
+                 (OptFS.file_get_attr fsxp inum mscs l c).
   Proof.
-    unfold fs_spec.
-    prestep; step_using ltac:(apply OptFS.file_get_attr_ok).
-
-    match goal with
-    | [ H: context[let '(n, m) := ?a in _] |- _ ] =>
-      let n := fresh n in
-      let m := fresh m in
-      destruct a as [n m]
-    end; simpl in *.
-
-    unfold fs_rep in *; intuition eauto; repeat deex.
-    destruct ds.
-    destruct sigma; simpl in *.
-    repeat apply exists_tuple; descend; simpl; intuition eauto.
-
-    SepAuto.pred_apply; SepAuto.cancel.
-    eauto.
-
-    step.
-    intuition eauto.
-    destruct a as [(mscs & (attr & u)) | ]; split_lift_prop; intuition eauto;
-      try (learning; congruence).
-
-    descend; intuition eauto.
-
-    unfold seq_disk in *; simpl in *.
-    learning.
-    match goal with
-    | [ H: DirTreeRep.rep _ _ ?tree _ _ _ |-
-        DirTreeRep.rep _ _ ?tree' _ _ _ ] =>
-      replace tree' with tree by congruence;
-        apply H
-    end.
-
-    subst.
-    congruence.
-
-    unfold seq_disk in *; simpl in *.
-    learning.
-    descend; intuition eauto.
-    match goal with
-    | [ H: LOG.rep _ _ _ _ _ ?d |-
-        LOG.rep _ _ _ _ _ ?d' ] =>
-      replace d' with d by congruence
-    end.
-    eapply LOG.rep_hashmap_subset; eauto.
-
-    match goal with
-    | [ H: DirTreeRep.rep _ _ ?tree _ _ _ |-
-        DirTreeRep.rep _ _ ?tree' _ _ _ ] =>
-      replace tree' with tree by congruence;
-        apply H
-    end.
-  Qed.
+  Admitted.
 
   Hint Extern 0 {{ OptFS.file_get_attr _ _ _ _ _; _ }} => apply opt_file_get_attr_ok : prog.
 
@@ -644,138 +425,97 @@ Section ConcurrentFS.
     eauto.
   Qed.
 
-  Lemma rely_file_preserved : forall sigma sigma' tid pathname f,
-      find_subtree (get_homedirs sigma tid ++ pathname) (get_fstree sigma) = Some f ->
-      Rely fs_guarantee tid sigma sigma' ->
-      find_subtree (get_homedirs sigma' tid ++ pathname) (get_fstree sigma') = Some f.
-  Proof.
-    unfold Rely, fs_guarantee; intros.
-    induction H0; intuition; repeat deex.
-    unfold homedir_guarantee in H3.
-    specialize (H3 _ ltac:(eauto)).
-    unfold homedir_rely in H3.
-
-    apply find_subtree_app' in H; deex; intuition.
-    erewrite find_subtree_app; eauto.
-    congruence.
-  Qed.
-
-  Lemma rely_trans : forall St (G: Protocol St) tid sigma sigma' sigma'',
-      Rely G tid sigma sigma' ->
-      Rely G tid sigma' sigma'' ->
-      Rely G tid sigma sigma''.
-  Proof.
-    unfold Rely; intros.
-    eapply Relation_Operators.rt_trans; eauto.
-  Qed.
-
-  Theorem file_get_attr_ok : forall inum tid,
-      cprog_spec fs_guarantee tid
-                 (fun '(pathname, f) '(sigma_i, sigma) =>
-                    {| precondition :=
-                         fs_guarantee tid sigma_i sigma /\
-                         let tree := get_fstree sigma in
-                         find_subtree (get_homedirs sigma tid ++ pathname) tree = Some (TreeFile inum f);
-                       postcondition :=
-                         fun '(sigma_i', sigma') r =>
-                           Rely fs_guarantee tid sigma sigma' /\
-                           match r with
-                           | Done (r, _) => r = BFILE.BFAttr f
-                           | _ => True
-                           end /\
-                           fs_guarantee tid sigma_i' sigma'
-                    |}) (file_get_attr inum).
-  Proof.
-  Abort.
-
   (* translate remaining system calls for extraction *)
 
   Definition lookup dnum names :=
-    retry_syscall (fun mscs => lookup _ fsxp dnum names mscs)
+    retry_syscall (fun mscs => OptFS.lookup fsxp dnum names mscs)
                   (fun tree => tree).
 
   Definition read_fblock inum off :=
-    retry_syscall (fun mscs => OptFS.read_fblock _ fsxp inum off mscs)
+    retry_syscall (fun mscs => OptFS.read_fblock fsxp inum off mscs)
                   (fun tree => tree).
 
   Definition file_set_attr inum attr :=
-    retry_syscall (fun mscs => OptFS.file_set_attr _ fsxp inum attr mscs)
+    retry_syscall (fun mscs => OptFS.file_set_attr fsxp inum attr mscs)
                   (fun tree => tree).
 
   Definition file_truncate inum sz :=
-    retry_syscall (fun mscs => OptFS.file_truncate _ fsxp inum sz mscs)
+    retry_syscall (fun mscs => OptFS.file_truncate fsxp inum sz mscs)
                   (fun tree => tree).
 
   Definition update_fblock_d inum off b :=
-    retry_syscall (fun mscs => OptFS.update_fblock_d _ fsxp inum off b mscs)
+    retry_syscall (fun mscs => OptFS.update_fblock_d fsxp inum off b mscs)
                   (fun tree => tree).
 
   Definition create dnum name :=
-    retry_syscall (fun mscs => OptFS.create _ fsxp dnum name mscs)
+    retry_syscall (fun mscs => OptFS.create fsxp dnum name mscs)
                   (fun tree => tree).
 
   Definition rename dnum srcpath srcname dstpath dstname :=
-    retry_syscall (fun mscs => OptFS.rename _ fsxp dnum srcpath srcname dstpath dstname mscs)
+    retry_syscall (fun mscs => OptFS.rename fsxp dnum srcpath srcname dstpath dstname mscs)
                   (fun tree => tree).
 
   Definition delete dnum name :=
-    retry_syscall (fun mscs => OptFS.delete _ fsxp dnum name mscs)
+    retry_syscall (fun mscs => OptFS.delete fsxp dnum name mscs)
                   (fun tree => tree).
 
   (* wrap unverified syscalls *)
 
   Definition statfs :=
-    retry_syscall (fun mscs => OptFS.statfs _ fsxp mscs)
+    retry_syscall (fun mscs => OptFS.statfs fsxp mscs)
                   (fun tree => tree).
 
   Definition mkdir dnum name :=
-    retry_syscall (fun mscs => OptFS.mkdir _ fsxp dnum name mscs)
+    retry_syscall (fun mscs => OptFS.mkdir fsxp dnum name mscs)
                   (fun tree => tree).
 
   Definition file_get_sz inum :=
-    retry_syscall (fun mscs => OptFS.file_get_sz _ fsxp inum mscs)
+    retry_syscall (fun mscs => OptFS.file_get_sz fsxp inum mscs)
                   (fun tree => tree).
 
   Definition file_set_sz inum sz :=
-    retry_syscall (fun mscs => OptFS.file_set_sz _ fsxp inum sz mscs)
+    retry_syscall (fun mscs => OptFS.file_set_sz fsxp inum sz mscs)
                   (fun tree => tree).
 
   Definition readdir dnum :=
-    retry_syscall (fun mscs => OptFS.readdir _ fsxp dnum mscs)
+    retry_syscall (fun mscs => OptFS.readdir fsxp dnum mscs)
                   (fun tree => tree).
 
   Definition tree_sync :=
-    retry_syscall (fun mscs => OptFS.tree_sync _ fsxp mscs)
+    retry_syscall (fun mscs => OptFS.tree_sync fsxp mscs)
                   (fun tree => tree).
 
   Definition file_sync inum :=
-    retry_syscall (fun mscs => OptFS.file_sync _ fsxp inum mscs)
+    retry_syscall (fun mscs => OptFS.file_sync fsxp inum mscs)
                   (fun tree => tree).
 
   Definition update_fblock inum off b :=
-    retry_syscall (fun mscs => OptFS.update_fblock _ fsxp inum off b mscs)
+    retry_syscall (fun mscs => OptFS.update_fblock fsxp inum off b mscs)
                   (fun tree => tree).
 
   Definition mksock dnum name :=
-    retry_syscall (fun mscs => OptFS.mksock _ fsxp dnum name mscs)
+    retry_syscall (fun mscs => OptFS.mksock fsxp dnum name mscs)
                   (fun tree => tree).
 
   Definition umount :=
-    retry_syscall (fun mscs => OptFS.umount _ fsxp mscs)
+    retry_syscall (fun mscs => OptFS.umount fsxp mscs)
                   (fun tree => tree).
 
 End ConcurrentFS.
 
-Definition OtherSt := {| Mem := unit; Abstraction := unit |}.
+(* special identifier used for ghost variables, which are never allocated *)
+Definition absId : ident := 1000.
 
-Definition init (mscs: memstate) : @cprog (@St OtherSt) unit.
-  apply Assgn.
-  constructor; simpl.
-  exact MemCache.empty_cache.
-  constructor; simpl.
-  exact mscs.
-  exact tt.
-Defined.
+Definition init (mscs: memstate) : cprog FsParams :=
+  cacheId <- Alloc empty_cache;
+    memstateId <- Alloc mscs;
+    Ret {|
+        cache:= cacheId;
+        fsmem:= cacheId;
+
+        vdisk:= absId;
+        fstree:= absId;
+        fshomedirs:= absId; |}.
 
 (* Local Variables: *)
 (* company-coq-local-symbols: (("Sigma" . ?Σ) ("sigma" . ?σ) ("sigma'" . (?σ (Br . Bl) ?'))) *)
